pure/Learn.Util.fst
@@ -9,6 +9,8 @@ let hide_propI_by p prf = prf ()
 
 let hide_propD p = ()
 
+let f_equal #a #b f x y = ()
+
 let prop_equal #a p x y = ()
 
 let assert_by p prf = prf ()
